theories/examples/factorial.v
@@ -1,0 +1,167 @@
+(* Show how an imperative factorial refines a functional one
+- Read a number from a tape
+- Compute factorial
+- ????
+- REFINEMENT!!!111
+
+ *)
+From Equations Require Import Equations.
+From gitrees Require Import gitree.
+From gitrees.input_lang Require Import lang interp.
+From gitrees.examples Require Import store while.
+
+
+(* #[local] Definition V1 : var [();()] := Vs Vz. *)
+#[local] Notation V1 := (Vs Vz).
+Definition fact_expr : expr [].
+Proof.
+  refine (Rec (If (Var V1) (Val $ Lit 1)
+                 (NatOp lang.Add (Var V1)
+                    (App (Var Vz) (NatOp lang.Sub (Var V1) (Val $ Lit 1)))))).
+Defined.
+
+Section fact.
+  Definition rs : gReifiers 2 :=
+    gReifiers_cons reify_input (gReifiers_cons reify_store gReifiers_nil).
+  Notation F := (gReifiers_ops rs).
+  Notation IT := (IT F).
+  Notation ITV := (ITV F).
+
+  Context `{!invGS Σ, !stateG rs Σ, !heapG rs Σ}.
+  Notation iProp := (iProp Σ).
+
+  (* XXX : why do we need reifiers for this? *)
+  Definition fact_fun : IT := interp_expr rs fact_expr ().
+
+  Lemma wp_seq α β Φ `{!NonExpansive Φ} :
+    WP@{rs} α {{ _, WP@{rs} β {{ Φ }} }} ⊢ WP@{rs} (SEQ α β) {{ Φ }}.
+  Proof.
+    iIntros "H".
+    iApply (wp_bind _ (SEQCtx β)).
+    iApply (wp_wand with "H").
+    iIntros (?) "Hb". unfold SEQCtx.
+    by rewrite SEQ_Val.
+  Qed.
+  Lemma wp_let α (f : IT -n> IT) Φ `{!NonExpansive Φ} :
+    WP@{rs} α {{ αv, WP@{rs} f (IT_of_V αv) {{ Φ }} }} ⊢ WP@{rs} (LET α f) {{ Φ }}.
+  Proof.
+    iIntros "H".
+    iApply (wp_bind _ (LETCTX f)).
+    iApply (wp_wand with "H").
+    iIntros (?) "Hb". simpl.
+    by rewrite LET_Val.
+  Qed.
+
+  Opaque ALLOC READ WRITE.
+  Program Definition fact_imp_body (n : nat) (acc ℓ : loc) : IT :=
+    WHILE (READ ℓ) $
+         LET (READ ℓ) $ λne i,
+         LET (NATOP Nat.mul i (READ acc)) $ λne r,
+         LET (NATOP Nat.sub i (Nat 1)) $ λne i,
+         SEQ (WRITE acc r)
+             (WRITE ℓ i).
+  Solve All Obligations with first [ solve_proper | solve_proper_please ].
+  (* XXX: this can be faster *)
+
+  Program Definition fact_imp : IT := λit n,
+    flip get_nat n $ λ n,
+    ALLOC (Nat 1) $ λne acc,
+    ALLOC (Nat n) $ λne ℓ,
+      SEQ
+        (fact_imp_body n acc ℓ)
+        (READ acc).
+
+  Lemma wp_fact_imp_bod n m acc ℓ :
+    heap_ctx -∗
+    pointsto acc (Nat m) -∗ pointsto ℓ (Nat n) -∗
+    WP@{rs} fact_imp_body n acc ℓ {{ _, pointsto acc (Nat (m * fact n)) }}.
+  Proof.
+    iIntros "#Hctx Hacc Hl".
+    iLöb as "IH" forall (n m).
+    unfold fact_imp_body.
+    rewrite {2}(WHILE_eq (READ _)).
+    iApply (wp_bind rs (IFSCtx _ (Nat 0)) (READ ℓ)).
+    iApply (wp_read with "Hctx Hl").
+    iNext. iNext. iIntros "Hl".
+    iApply wp_val. iModIntro.
+    unfold IFSCtx. simpl.
+    destruct n as [|n].
+    - rewrite IF_False; last lia.
+      iApply wp_val. simpl. rewrite Nat.mul_1_r//.
+    - rewrite IF_True; last lia.
+      iApply wp_seq.
+      iApply wp_let.
+      iApply (wp_read with "Hctx Hl").
+      iNext. iNext. iIntros "Hl".
+      iApply wp_val. simpl.
+      iApply wp_let.
+      iApply (wp_bind _ (NatOpRSCtx _ (Nat (S n)))).
+      { solve_proper_please. }
+      iModIntro.
+      iApply (wp_read with "Hctx Hacc").
+      iNext. iNext. iIntros "Hacc".
+      iApply wp_val. iModIntro.
+      simpl. unfold NatOpRSCtx.
+      rewrite NATOP_Nat.
+      iApply wp_val. iModIntro.
+      iApply wp_let.
+      rewrite NATOP_Nat.
+      iApply wp_val. iModIntro.
+      simpl.
+      iApply wp_seq.
+      iApply (wp_write with "Hctx Hacc").
+      iNext. iNext. iIntros "Hacc".
+      iApply (wp_write with "Hctx Hl").
+      iNext. iNext. iIntros "Hl".
+      iApply wp_tick. iNext.
+      replace (m + n*m) with ((n + 1) * m) by lia.
+      iSpecialize ("IH" with "Hacc  Hl" ).
+      iApply (wp_wand with "IH").
+      iIntros (_).
+      rewrite Nat.sub_0_r.
+      replace ((n + 1) * m * fact n) with (m * (fact n + n * fact n)) by lia.
+      iIntros "$". done.
+  Qed.
+
+  Lemma wp_fact_imp (n : nat) :
+    heap_ctx ⊢ WP@{rs} fact_imp ⊙ (Nat n) {{  βv, βv ≡ NatV (fact n)  }}.
+  Proof.
+    iIntros "#Hctx".
+    rewrite APP'_Fun_l/=. rewrite -Tick_eq.
+    iApply wp_tick.
+    iNext. rewrite get_nat_nat.
+    iApply (wp_alloc with "Hctx").
+    { solve_proper. }
+    fold rs. iNext. iNext.
+    iIntros (acc) "Hacc". simpl.
+    iApply (wp_alloc with "Hctx").
+    { solve_proper. }
+    fold rs. iNext. iNext.
+    iIntros (ℓ) "Hl". simpl.
+    iApply wp_seq.
+    { solve_proper. }
+    iApply (wp_wand _ _ _ _ (λ _, pointsto acc (Nat $ fact n)) with "[-]"); last first.
+    { simpl. iIntros (_) "Hacc".
+      iModIntro. iApply (wp_read with "Hctx Hacc").
+      iNext. iNext. iIntros "Hacc".
+      iApply wp_val. done. }
+    iPoseProof (wp_fact_imp_bod with "Hctx Hacc Hl") as "H".
+    by rewrite Nat.mul_1_l.
+  Qed.
+
+  Program Definition fact_combined : IT :=
+    INPUT $ λne n, fact_imp ⊙ (Nat n).
+  Lemma wp_fact_combined (n : nat) :
+    heap_ctx ∗ has_substate (State [n])
+    ⊢ WP@{rs} fact_combined {{  βv, βv ≡ NatV (fact n)  }}.
+  Proof.
+    iIntros "[#Hctx Htape]".
+    unfold fact_combined.
+    iApply (wp_input with "Htape").
+    { reflexivity. }
+    iNext. iIntros "_ Htape".
+    simpl. iApply (wp_fact_imp with "Hctx").
+  Qed.
+
+End fact.
+
