theories/examples/while.v
@@ -1,0 +1,21 @@
+From gitrees Require Import prelude gitree.
+
+Section while.
+  Context {E : opsInterp}.
+  Notation IT := (IT E).
+  Notation ITV := (ITV E).
+
+  Program Definition pre_while (while : IT -n> IT -n> IT) : IT -n> IT -n> IT :=
+    λne cond body, IF cond (SEQ body (Tick (while cond body))) (Nat 0).
+  Solve All Obligations with solve_proper_please.
+
+  #[local] Instance pre_while_contractive : Contractive pre_while.
+  Proof. solve_contractive. Qed.
+  Definition WHILE : IT -n> IT -n> IT := fixpoint pre_while.
+
+  (** WHILE (α > 0) DO β *)
+  Lemma WHILE_eq α β :
+    WHILE α β ≡ IF α (SEQ β (Tick (WHILE α β))) (Nat 0).
+  Proof. apply (fixpoint_unfold pre_while _ _). Qed.
+
+End while.
